Reverting from using Definitions

Meta.v
@@ -5,39 +5,80 @@ From Elo Require Import Array.
 From Elo Require Import Core.
 From Elo Require Import CoreExt.
 
-(* ------------------------------------------------------------------------- *)
+(* ----------------------------------------------------------------------------
 
-Definition subst_preservation (P : mem -> tm -> Prop) :=
+(* Used by tstep_none_preservation *)
+subst_preservation:
   forall m t tx x,
     P m t ->
     P m tx ->
     P m ([x := tx] t).
 
-Definition mem_add_preservation (P : mem -> tm -> Prop) :=
+(* Used by tstep_alloc_preservation *)
+mem_add_preservation:
   forall m t vT,
     P m t ->
     P (m +++ vT) t.
 
-Definition mem_set_preservation (P : mem -> tm -> Prop) :=
-  forall m t ad v T,
+(* Used by tstep_write_preservation *)
+mem_set_preservation:
+  forall m t ad vT,
+    P m t ->
+    P m[ad <- vT] t.
+
+-------------------------------------------------------------------------------
+
+tstep_none_preservation:
+  forall m t t',
+    P m t ->
+    t --[EF_None]--> t' ->
+    P m t'.
+
+tstep_alloc_preservation:
+  forall m t t' v T,
+    P m t ->
+    t --[EF_Alloc (#m) v T]--> t' ->
+    P (m +++ (v, T)) t'.
+
+tstep_read_preservation:
+  forall m t t' ad v,
     P m v ->
     P m t ->
-    P m[ad <- (v, T)] t.
+    t --[EF_Read ad v]--> t' ->
+    P m t'.
 
-(* ------------------------------------------------------------------------- *)
+tstep_write_preservation:
+  forall m t t' ad v T,
+    P m t ->
+    t --[EF_Write ad v T]--> t' ->
+    P m[ad <- (v, T)] t'.
 
-Definition thread_default_preservation (P : mem -> tm -> Prop) :=
+tstep_spawn_preservation:
+  forall m t t' block,
+    P m t ->
+    t --[EF_Spawn block]--> t' ->
+    P m t'.
+
+mstep_preservation:
+  forall_memory m (P m) ->
+    P m t ->
+    m / t ==[e]==> m' / t' ->
+    P m' t'.
+
+-------------------------------------------------------------------------------
+
+thread_default_preservation:
   forall m,
     P m thread_default.
 
-Definition spawn_block_preservation (P : mem -> tm -> Prop) :=
+spawn_block_preservation:
   forall m t t' block,
     P m t ->
     t --[EF_Spawn block]--> t' ->
     P m block.
 
 (* The untouched threads with the new memory still preserve the property. *)
-Definition untouched_threads_preservation (P : mem -> tm -> Prop) :=
+untouched_threads_preservation:
   forall m m' ths tid tid' e t',
     forall_threads ths (P m) ->
     tid <> tid' ->
@@ -45,78 +86,118 @@ Definition untouched_threads_preservation (P : mem -> tm -> Prop) :=
     m / ths[tid] ==[e]==> m' / t' ->
     P m' ths[tid'].
 
-(* ------------------------------------------------------------------------- *)
-
-Definition tstep_none_preservation (P : mem -> tm -> Prop) :=
-  forall m t t',
-    P m t ->
-    t --[EF_None]--> t' ->
-    P m t'.
-
-Definition tstep_alloc_preservation (P : mem -> tm -> Prop) :=
-  forall m t t' v T,
-    P m t ->
-    t --[EF_Alloc (#m) v T]--> t' ->
-    P (m +++ (v, T)) t'.
-
-Definition tstep_read_preservation (P : mem -> tm -> Prop) :=
-  forall m t t' ad v,
-    P m v ->
-    P m t ->
-    t --[EF_Read ad v]--> t' ->
-    P m t'.
-
-Definition tstep_write_preservation (P : mem -> tm -> Prop) :=
-  forall m t t' ad v T,
-    P m t ->
-    t --[EF_Write ad v T]--> t' ->
-    P m[ad <- (v, T)] t'.
-
-Definition tstep_spawn_preservation (P : mem -> tm -> Prop) :=
-  forall m t t' block,
-    P m t ->
-    t --[EF_Spawn block]--> t' ->
-    P m t'.
-
-Definition mstep_preservation (P : mem -> tm -> Prop) :=
-  forall m m' t t' e,
-    forall_memory m (P m) ->
-    P m t ->
-    m / t ==[e]==> m' / t' ->
-    P m' t'.
-
-Definition cstep_preservation (P : mem -> tm -> Prop) :=
+cstep_preservation:
   forall m m' ths ths' tid e,
     forall_memory m (P m) ->
     forall_threads ths (P m) ->
     m / ths ~~[tid, e]~~> m' / ths' ->
     forall_threads ths' (P m').
 
-Definition property_preservation (P : mem -> tm -> Prop) :=
+-------------------------------------------------------------------------------
+
+tstep_alloc_mem_preservation:
+  forall m t t' v T,
+    P m t ->
+    forall_memory m (P m) ->
+    t --[EF_Alloc (#m) v T]--> t' ->
+    forall_memory  (m +++ (v, T)) (P (m +++ (v, T))).
+
+tstep_write_mem_preservation:
+  forall m t t' ad v T,
+    P m t ->
+    forall_memory m (P m) ->
+    t --[EF_Write ad v T]--> t' ->
+    forall_memory m[ad <- (v, T)] (P m[ad <- (v, T)]).
+
+mstep_mem_preservation:
+  forall m m' t t' e,
+    P m t ->
+    forall_memory m (P m) ->
+    m / t ==[e]==> m' / t' ->
+    forall_memory m' (P m').
+
+cstep_mem_preservation:
+  forall m m' ths ths' tid e,
+    forall_threads ths (P m) ->
+    forall_memory m (P m) ->
+    m / ths ~~[tid, e]~~> m' / ths' ->
+    forall_memory m' (P m').
+
+-------------------------------------------------------------------------------
+
+preservation:
   forall m m' ths ths' tid e,
     forall_program m ths (P m) ->
     m / ths ~~[tid, e]~~> m' / ths' ->
     forall_program m' ths' (P m').
 
-(* ------------------------------------------------------------------------- *)
+---------------------------------------------------------------------------- *)
 
-Corollary mstep_preserves (P : mem -> tm -> Prop) :
-  tstep_none_preservation P ->
-  tstep_alloc_preservation P ->
-  tstep_read_preservation P ->
-  tstep_write_preservation P ->
-  mstep_preservation P.
-Proof. unfold mstep_preservation. intros. inversion_mstep; eauto. Qed.
+Corollary mstep_preservation (P : mem -> tm -> Prop) :
+  (* tstep_none_preservation *)
+  (forall m t t',
+    P m t ->
+    t --[EF_None]--> t' ->
+    P m t') ->
+  (* tstep_alloc_preservation *)
+  (forall m t t' v T,
+    P m t ->
+    t --[EF_Alloc (#m) v T]--> t' ->
+    P (m +++ (v, T)) t') ->
+  (* tstep_read_preservation *)
+  (forall m t t' ad v,
+    P m v ->
+    P m t ->
+    t --[EF_Read ad v]--> t' ->
+    P m t') ->
+  (* tstep_write_preservation: *)
+  (forall m t t' ad v T,
+    P m t ->
+    t --[EF_Write ad v T]--> t' ->
+    P m[ad <- (v, T)] t') ->
+  (* What we want to prove: *)
+  forall m m' t t' e,
+    forall_memory m (P m) ->
+    P m t ->
+    m / t ==[e]==> m' / t' ->
+    P m' t'.
+Proof. intros. inversion_mstep; eauto. Qed.
 
-Lemma cstep_preserves (P : mem -> tm -> Prop) :
-    thread_default_preservation P ->
-    spawn_block_preservation P ->
-    untouched_threads_preservation P ->
-    mstep_preservation P ->
-    tstep_spawn_preservation P ->
-    cstep_preservation P.
+Lemma cstep_preservation (P : mem -> tm -> Prop) :
+    (* tstep_spawn_preservation *)
+    (forall m t t' block,
+      P m t ->
+      t --[EF_Spawn block]--> t' ->
+      P m t') ->
+    (* mstep_preservation *)
+    (forall m m' t t' e,
+      forall_memory m (P m) ->
+      P m t ->
+      m / t ==[e]==> m' / t' ->
+      P m' t') ->
+    (* thread_default_preservation *)
+    (forall m,
+      P m thread_default) ->
+    (* spawn_block_preservation *)
+    (forall m t t' block,
+      P m t ->
+      t --[EF_Spawn block]--> t' ->
+      P m block) ->
+    (* untouched_threads_preservation *)
+    (forall m m' ths tid tid' e t',
+      forall_threads ths (P m) ->
+      tid <> tid' ->
+      tid' < #ths ->
+      m / ths[tid] ==[e]==> m' / t' ->
+      P m' ths[tid']) ->
+    (* What we want to prove: *)
+    forall m m' ths ths' tid e,
+      forall_memory m (P m) ->
+      forall_threads ths (P m) ->
+      m / ths ~~[tid, e]~~> m' / ths' ->
+      forall_threads ths' (P m').
 Proof.
-  unfold cstep_preservation. intros. inversion_cstep; intros tid'.
+  intros. inversion_cstep; intros tid'.
   - destruct (nat_eq_dec tid' (#ths)); subst.
     + rewrite <- (set_preserves_length _ tid t'). simpl_array. eauto.
     + destruct (lt_eq_lt_dec tid' (length ths)) as [[Ha | ?] | Hb]; subst;
@@ -124,11 +205,64 @@ Proof.
       * rewrite <- (set_preserves_length _ tid t') in Ha. simpl_array.
         destruct (nat_eq_dec tid tid'); subst; simpl_array; eauto.
       * rewrite <- (set_preserves_length _ tid t') in Hb. simpl_array. eauto.
-  - destruct (nat_eq_dec tid tid'); subst; simpl_array;
-    eauto using (mstep_preserves P).
+  - destruct (nat_eq_dec tid tid'); subst; simpl_array; eauto.
     decompose sum (lt_eq_lt_dec tid' (#ths)); subst; eauto;
     simpl_array; eauto.
 Qed.
 
-#[export] Hint Resolve mstep_preserves cstep_preserves : preservation.
+Corollary mstep_mem_preservation (P : mem -> tm -> Prop) :
+  (* tstep_alloc_mem_preservation *)
+  (forall m t t' v T,
+    P m t ->
+    forall_memory m (P m) ->
+    t --[EF_Alloc (#m) v T]--> t' ->
+    forall_memory  (m +++ (v, T)) (P (m +++ (v, T)))) ->
+  (* tstep_write_mem_preservation *)
+  (forall m t t' ad v T,
+    P m t ->
+    forall_memory m (P m) ->
+    t --[EF_Write ad v T]--> t' ->
+    forall_memory m[ad <- (v, T)] (P m[ad <- (v, T)])) ->
+  (* What we want to prove: *)
+  forall m m' t t' e,
+    P m t ->
+    forall_memory m (P m) ->
+    m / t ==[e]==> m' / t' ->
+    forall_memory m' (P m').
+Proof. intros. inversion_mstep; eauto. Qed.
+
+Corollary cstep_mem_preservation (P : mem -> tm -> Prop) :
+  (* mstep_mem_preservation *)
+  (forall m m' t t' e,
+    P m t ->
+    forall_memory m (P m) ->
+    m / t ==[e]==> m' / t' ->
+    forall_memory m' (P m')) ->
+  (* What we want to prove: *)
+  forall m m' ths ths' tid e,
+    forall_threads ths (P m) ->
+    forall_memory m (P m) ->
+    m / ths ~~[tid, e]~~> m' / ths' ->
+    forall_memory m' (P m').
+Proof. intros. inversion_cstep; eauto. Qed.
+
+Corollary preservation (P : mem -> tm -> Prop) :
+  (* cstep_preservation *)
+  (forall m m' ths ths' tid e,
+    forall_memory m (P m) ->
+    forall_threads ths (P m) ->
+    m / ths ~~[tid, e]~~> m' / ths' ->
+    forall_threads ths' (P m')) ->
+  (* cstep_mem_preservation *)
+  (forall m m' ths ths' tid e,
+    forall_threads ths (P m) ->
+    forall_memory m (P m) ->
+    m / ths ~~[tid, e]~~> m' / ths' ->
+    forall_memory m' (P m')) ->
+  (* What we want to prove: *)
+  forall m m' ths ths' tid e,
+    forall_program m ths (P m) ->
+    m / ths ~~[tid, e]~~> m' / ths' ->
+    forall_program m' ths' (P m').
+Proof. intros ? ? * [? ?]. eauto. Qed.
 
