ValidAddresses.v
@@ -114,10 +114,11 @@ Local Lemma vad_spawn : forall m t,
   valid_addresses m <{ spawn t }>.
 Proof. eauto with has_address_inversion. Qed.
 
-Local Hint Resolve vad_unit vad_num 
-                   vad_new vad_load vad_asg
-                   vad_var vad_fun vad_call vad_seq vad_spawn
-                   : vad_constructors.
+Local Hint Resolve
+  vad_unit vad_num 
+  vad_new vad_load vad_asg
+  vad_var vad_fun vad_call vad_seq vad_spawn
+  : vad_constructors.
 
 (* ------------------------------------------------------------------------- *)
 (* inversion                                                                 *)
@@ -187,120 +188,137 @@ Ltac inversion_vad :=
 (* preservation                                                              *)
 (* ------------------------------------------------------------------------- *)
 
-Local Lemma subst_preservation_vad :
-  subst_preservation valid_addresses.
+Local Lemma vad_subst_preservation : forall m t tx x,
+  valid_addresses m t ->
+  valid_addresses m tx ->
+  valid_addresses m ([x := tx] t).
 Proof.
-  unfold subst_preservation.
   intros. induction t; try inversion_vad; simpl; eauto with vad_constructors;
   destruct string_eq_dec; subst; trivial;
   autounfold in *; eauto with has_address_inversion.
-Qed.
+Defined.
 
-Local Lemma mem_add_preservation_vad :
-  mem_add_preservation valid_addresses.
+Local Lemma vad_mem_add_preservation : forall m t vT,
+  valid_addresses m t ->
+  valid_addresses (m +++ vT) t.
 Proof.
-  unfold mem_add_preservation.
   intros. intros ? Hha. rewrite add_increments_length.
   induction Hha; try inversion_vad; eauto with has_address_inversion.
 Qed.
 
-Local Lemma mem_set_preservation_vad :
-  mem_set_preservation valid_addresses.
+Local Lemma vad_mem_set_preservation : forall m t ad vT,
+  valid_addresses m t ->
+  valid_addresses m[ad <- vT] t.
 Proof.
-  unfold mem_set_preservation.
   intros. intros ? Hha. rewrite set_preserves_length.
   induction Hha; try inversion_vad; eauto with has_address_inversion.
 Qed.
 
 (* ------------------------------------------------------------------------- *)
 
-Local Lemma thread_default_preservation_vad :
-  thread_default_preservation valid_addresses.
+Local Lemma vad_tstep_none_preservation : forall m t t',
+  valid_addresses m t ->
+  t --[EF_None]--> t' ->
+  valid_addresses m t'.
 Proof.
-  unfold thread_default_preservation.
+  intros. induction_step; inversion_vad; eauto with vad_constructors. 
+  inversion_vad. eauto using vad_subst_preservation.
+Qed.
+
+Local Lemma vad_tstep_alloc_preservation : forall m t t' v T,
+  valid_addresses m t ->
+  t --[EF_Alloc (#m) v T]--> t' ->
+  valid_addresses (m +++ (v, T)) t'.
+Proof.
+  intros. induction_step; inversion_vad;
+  eauto using vad_mem_add_preservation with vad_constructors.
+  intros ? ?. inversion_has_address. rewrite add_increments_length. eauto.
+Qed.
+
+Local Lemma vad_tstep_read_preservation : forall m t t' ad v,
+  valid_addresses m v ->
+  valid_addresses m t ->
+  t --[EF_Read ad v]--> t' ->
+  valid_addresses m t'.
+Proof.
+  intros. induction_step; inversion_vad; eauto with vad_constructors.
+Qed.
+
+Local Lemma vad_tstep_write_preservation : forall m t t' ad v T,
+  valid_addresses m t ->
+  t --[EF_Write ad v T]--> t' ->
+  valid_addresses m[ad <- (v, T)] t'.
+Proof.
+  intros. assert (valid_addresses m v); induction_step; inversion_vad;
+  eauto using vad_mem_set_preservation with vad_constructors.
+Qed.
+
+Local Lemma vad_tstep_spawn_preservation : forall m t t' block,
+  valid_addresses m t ->
+  t --[EF_Spawn block]--> t' ->
+  valid_addresses m t'.
+Proof.
+  intros. induction_step; inversion_vad; eauto with vad_constructors.
+Qed.
+
+Local Corollary vad_mstep_preservation : forall m m' t t' e,
+  forall_memory m (valid_addresses m) ->
+  valid_addresses m t ->
+  m / t ==[e]==> m' / t' ->
+  valid_addresses m' t'.
+Proof.
+  eauto 6 using (mstep_preservation valid_addresses),
+    vad_tstep_none_preservation,
+    vad_tstep_alloc_preservation,
+    vad_tstep_read_preservation,
+    vad_tstep_write_preservation.
+Qed.
+
+(* ------------------------------------------------------------------------- *)
+
+Local Lemma vad_thread_default_preservation : forall m,
+  valid_addresses m thread_default.
+Proof.
   intros. intros ? ?. inversion_has_address.
 Qed.
 
-Local Lemma spawn_block_preservation_vad :
-  spawn_block_preservation valid_addresses.
+Local Lemma vad_spawn_block_preservation : forall m t t' block,
+  valid_addresses m t ->
+  t --[EF_Spawn block]--> t' ->
+  valid_addresses m block.
 Proof.
-  unfold spawn_block_preservation.
   intros. induction_step; inversion_vad; eauto.
 Qed.
 
-Local Lemma untouched_threads_preservation_vad :
-  untouched_threads_preservation valid_addresses.
+Local Lemma vad_untouched_threads_preservation : forall m m' ths tid tid' e t',
+  forall_threads ths (valid_addresses m) ->
+  tid <> tid' ->
+  tid' < #ths ->
+  m / ths[tid] ==[e]==> m' / t' ->
+  valid_addresses m' ths[tid'].
 Proof.
-  unfold untouched_threads_preservation.
   intros. intros ? ?. autounfold in *. inversion_mstep; eauto;
   (rewrite add_increments_length || rewrite set_preserves_length);
   eauto using Nat.lt_lt_succ_r.
 Qed.
 
+Local Corollary vad_cstep_preservation : forall m m' ths ths' tid e,
+  forall_memory m (valid_addresses m) ->
+  forall_threads ths (valid_addresses m) ->
+  m / ths ~~[tid, e]~~> m' / ths' ->
+  forall_threads ths' (valid_addresses m').
+Proof.
+  eauto 6 using cstep_preservation,
+    vad_tstep_spawn_preservation,
+    vad_mstep_preservation,
+    vad_thread_default_preservation,
+    vad_spawn_block_preservation,
+    vad_untouched_threads_preservation.
+Qed.
+
 (* ------------------------------------------------------------------------- *)
 
-Local Lemma tstep_none_preservation_vad :
-  tstep_none_preservation valid_addresses.
-Proof.
-  unfold tstep_none_preservation.
-  intros. induction_step; inversion_vad; eauto with vad_constructors. 
-  inversion_vad. eauto using subst_preservation_vad.
-Qed.
-
-Local Lemma tstep_alloc_preservation_vad :
-  tstep_alloc_preservation valid_addresses.
-Proof.
-  unfold tstep_alloc_preservation.
-  intros. induction_step; inversion_vad;
-  eauto using mem_add_preservation_vad with vad_constructors.
-  intros ? ?. rewrite add_increments_length. inversion_has_address. lia.
-Qed.
-
-Local Lemma tstep_read_preservation_vad :
-  tstep_read_preservation valid_addresses.
-Proof.
-  unfold tstep_read_preservation.
-  intros. induction_step; inversion_vad; eauto with vad_constructors.
-Qed.
-
-Local Lemma tstep_write_preservation_vad :
-  tstep_write_preservation valid_addresses.
-Proof.
-  unfold tstep_write_preservation.
-  intros. assert (valid_addresses m v); induction_step; inversion_vad;
-  eauto using mem_set_preservation_vad with vad_constructors.
-Qed.
-
-Local Lemma tstep_spawn_preservation_vad :
-  tstep_spawn_preservation valid_addresses.
-Proof.
-  unfold tstep_spawn_preservation.
-  intros. induction_step; inversion_vad; eauto with vad_constructors.
-Qed.
-
-Local Hint Resolve
-  subst_preservation_vad
-  mem_add_preservation_vad
-  mem_set_preservation_vad
-  thread_default_preservation_vad
-  spawn_block_preservation_vad
-  untouched_threads_preservation_vad
-  tstep_none_preservation_vad
-  tstep_alloc_preservation_vad
-  tstep_read_preservation_vad
-  tstep_write_preservation_vad
-  tstep_spawn_preservation_vad
-  : vad_preservation.
-
-Local Corollary cstep_preservation_vad :
-  cstep_preservation valid_addresses.
-Proof. eauto with preservation vad_preservation. Qed.
-
-(* ------------------------------------------------------------------------- *)
-(* memory preservation                                                       *)
-(* ------------------------------------------------------------------------- *)
-
-Local Lemma step_alloc_mem_vad_preservation : forall m t t' v T,
+Local Lemma vad_tstep_alloc_mem_preservation : forall m t t' v T,
   valid_addresses m t ->
   forall_memory m (valid_addresses m) ->
   t --[EF_Alloc (#m) v T]--> t' ->
@@ -313,7 +331,7 @@ Proof.
         with has_address_inversion.
 Qed.
 
-Local Lemma step_write_mem_vad_preservation : forall m t t' ad v T,
+Local Lemma vad_tstep_write_mem_preservation : forall m t t' ad v T,
   valid_addresses m t ->
   forall_memory m (valid_addresses m) ->
   t --[EF_Write ad v T]--> t' ->
@@ -321,36 +339,38 @@ Local Lemma step_write_mem_vad_preservation : forall m t t' ad v T,
 Proof.
   intros. intros ad'. 
   assert (ad < #m) by eauto using valid_address_write.
-  destruct (Nat.eq_dec ad ad'); subst; simpl_array;
+  destruct (eq_nat_dec ad ad'); subst; simpl_array;
   intros ? ?; rewrite set_preserves_length; autounfold in *;
   eauto using anyt_write_generalization, Nat.lt_lt_succ_r.
 Qed.
 
-Local Corollary mstep_mem_vad_preservation : forall m m' t t' e,
+Local Corollary vad_mstep_mem_preservation : forall m m' t t' e,
   valid_addresses m t ->
   forall_memory m (valid_addresses m) ->
   m / t ==[e]==> m' / t' ->
   forall_memory m' (valid_addresses m').
 Proof.
-  intros. inversion_mstep; trivial;
-  eauto using step_alloc_mem_vad_preservation, step_write_mem_vad_preservation.
+  eauto using mstep_mem_preservation,
+    vad_tstep_alloc_mem_preservation,
+    vad_tstep_write_mem_preservation.
+Qed.
+
+Local Corollary vad_cstep_mem_preservation : forall m m' ths ths' tid e,
+  forall_threads ths (valid_addresses m) ->
+  forall_memory m (valid_addresses m) ->
+  m / ths ~~[tid, e]~~> m' / ths' ->
+  forall_memory m' (valid_addresses m').
+Proof.
+  eauto using cstep_mem_preservation, vad_mstep_mem_preservation.
 Qed.
 
 (* ------------------------------------------------------------------------- *)
 
-Theorem valid_addresses_memory_preservation : forall m m' ths ths' tid e,
-  forall_memory m (valid_addresses m) ->
-  forall_threads ths (valid_addresses m) ->
+Theorem valid_addresses_preservation : forall m m' ths ths' tid e,
+  forall_program m ths (valid_addresses m) ->
   m / ths ~~[tid, e]~~> m' / ths' ->
-  forall_memory m' (valid_addresses m').
+  forall_program m' ths' (valid_addresses m').
 Proof.
-  intros. inversion_cstep; eauto using mstep_mem_vad_preservation.
-Qed.
-
-Corollary valid_addresses_preservation :
-  property_preservation valid_addresses.
-Proof.
-  unfold property_preservation. intros * [? ?] ?.
-  eauto using cstep_preservation_vad, valid_addresses_memory_preservation.
+  eauto using preservation, vad_cstep_preservation, vad_cstep_mem_preservation.
 Qed.
 
